compiler/backend/serialiser/README.md
@@ -1,0 +1,8 @@
+Proofs and automation for serialising HOL values.
+
+[backend_enc_decScript.sml](backend_enc_decScript.sml):
+Encoders and decoders to/from types configuration types in backend.
+
+[num_list_enc_decScript.sml](num_list_enc_decScript.sml):
+Encoders and decoders to/from types represented as prefixes of lists
+of natural numbers.
